is_stratified 류의 판별함수를, 재귀함수를 통해 정의하는 것에 계속 실패한다. Terminate 를 증명하지 못했다고. 어쩌면 좋지?

src/study/Nemonuri.Study.CSharpSyntaxRewriter2.Modifier/Nemonuri.GreenNode.fst
@@ -9,7 +9,7 @@ type green_node_schema (#t:Type) = {
   children:(list (green_node_schema #t))
 }
 
-let is_stratified (#t:Type) (gns:green_node_schema #t) : Tot bool =
+let rec is_stratified (#t:Type) (gns:green_node_schema #t) : Tot bool =
   if gns.level = 0 then 
     L.isEmpty gns.children
   else
@@ -18,13 +18,62 @@ let is_stratified (#t:Type) (gns:green_node_schema #t) : Tot bool =
       let v1 = L.map (fun (v2:green_node_schema #t) -> v2.level) gns.children in
       let v3 = LT.max_for_unempty_list v1 LT.default_int_comparer in
       v3 = gns.level - 1
+    ) &&
+    (
+      L.for_all (fun (v4:green_node_schema #t) -> is_stratified v4) gns.children
     )
 
-let has_type_green_node (#t:Type) (gns:green_node_schema #t) : Tot bool = is_stratified gns
+let is_self_level_greater_then_children (#t:Type) (gns:green_node_schema #t) : Tot bool =
+  if gns.level = 0 then 
+    L.isEmpty gns.children
+  else
+    L.for_all (fun (gns2:green_node_schema #t) -> gns2.level < gns.level) gns.children
+
+(*
+let rec is_weakly_stratified (#t:Type) (gns:green_node_schema #t) 
+  : Tot bool (decreases gns.level) =
+  (is_self_level_greater_then_children gns) &&
+  (
+    let children = gns.children in
+    (L.for_all (fun (gns2:green_node_schema #t) -> is_self_level_greater_then_children gns2) children) &&
+    (L.for_all (fun (gns2:green_node_schema #t) -> is_weakly_stratified gns2) children)
+  )
+*)
+
+let rec is_weakly_stratified (#t:Type) (gns:green_node_schema #t) : Tot bool =
+  if gns.level = 0 then 
+    L.isEmpty gns.children
+  else
+    let children = gns.children in
+      if L.isEmpty children then 
+        true
+      else
+        if L.for_all (fun (gns2:green_node_schema #t) -> gns2.level < gns.level) children then
+          L.for_all (fun (gns2:green_node_schema #t) -> is_weakly_stratified gns2) children
+        else
+          false
+
+(*
+let has_type_green_node (#t:Type) (gns:green_node_schema #t) : Tot bool = is_weakly_stratified gns
 let green_node (#t:Type) = gns:(green_node_schema #t){has_type_green_node gns}
 
 let has_type_green_leaf (#t:Type) (gn:green_node #t) : Tot bool =
   L.isEmpty gn.children
 let green_leaf (#t:Type) = gn:(green_node #t){has_type_green_leaf gn}
 
-let assert_level_of_green_leaf_is_zero = assert ( forall (t:Type) (gl:green_leaf #t). gl.level = 0 )
+let rec get_height (#t:Type) (gn:green_node #t)
+  : Tot nat (decreases gn.level) =
+  if has_type_green_leaf gn then 0
+  else
+    let v1 = L.map (fun (v2:green_node #t) -> get_height v2) gn.children in
+    let v3 = LT.max_for_unempty_list v1 LT.default_int_comparer in
+    v3 + 1
+*)
+
+// let assert_level_of_green_leaf_is_zero = assert ( forall (t:Type) (gl:green_leaf #t). gl.level = 0 )
+
+(*
+let assert_green_node_is_weak_green_node = assert ( 
+  forall (t:Type) (gn:green_node #t). (has_type_weak_green_node gn)
+)
+*)
